fixed proofs in polycomdl

PolyComDL.ec
@@ -38,7 +38,7 @@ clone export PolynomialCommitment as PolyComDL with
 abbrev ( ^ ) = Bl.ZP.( ^ ).
 
 
-(*fixed*) (*
+(*fixed*)
 lemma prod_sum_eq (a : exp) m :
     foldr Bl.GB.( * ) Bl.GB.e
       (mkseq (fun (i : int) => Bl.GB.g ^ (nth a m i)) (size m)) =
@@ -62,7 +62,7 @@ proof.
     apply (eq_from_nth Bl.GB.g). smt(@List). move => i hi.
     rewrite size_mkseq in hi. rewrite nth_mkseq. smt(). rewrite nth_mkseq. smt().
     simplify. smt(@List).
-qed. *)
+qed. 
 
 
 
@@ -79,7 +79,7 @@ qed. *)
   (* We first want to prove we can rephrase the combination of mkKey and prodEx in
             a way more favorable to induction *)
 
-      (*
+     
 (*fixed*)
 lemma mkKey_ga a : nth Bl.GB.g (Bl.mkKey a) 1 = Bl.GB.g ^ a.
 proof.
@@ -247,7 +247,7 @@ proof.
   simplify. trivial. 
 qed.
 
-  (* Now we are ready to define the main commitment scheme *) *)
+  (* Now we are ready to define the main commitment scheme *) 
 
  (* PK = g, g^α, . . . , g^α^t *)(*fixed*)
  module PolyComDLScheme : PC_Scheme = {
@@ -308,9 +308,14 @@ qed.
   }
 
 }.
-(*
-(*fixed*) 
- lemma PolyComDLScheme_Correctness : (* This always holds *)
+
+
+
+
+
+
+(*fixed*)
+lemma PolyComDLScheme_Correctness :
   hoare[Correctness(PolyComDLScheme).main : true ==> res].
 proof.
   proc. inline *. wp. rnd. auto. progress.
@@ -325,53 +330,56 @@ proof.
               <= max (deg p{hr}) (deg (polyC (peval p{hr} i{hr}))).
   + smt(@BasePoly).
   smt(Bl.t_valid).
-  simplify. 
+  simplify.
   rewrite Bl.e_pow1. rewrite Bl.e_g_g. rewrite mkKey_ga.
   rewrite -Bl.ZP.expB.
   rewrite Bl.e_pow1. rewrite Bl.e_pow2. rewrite Bl.e_g_g.
   rewrite -Bl.ZP_GT.expM.
-  rewrite -Bl.ZP_GT.expD. admit. (*
-  apply (Bl.GT_exp_polyid_bridge a i{hr}
-            (peval (edivpoly (p{hr} - polyC (peval p{hr} i{hr}))
-                              (X - polyC i{hr})).`1 a)
-            (peval p{hr} a)
-            (peval p{hr} i{hr})).
-have psi_eq :
-    (edivpoly (p{hr} - polyC (peval p{hr} i{hr})) (X - polyC i{hr})).`1
-  = (edivpoly p{hr} (X - polyC i{hr})).`1.
-+ apply (ediv_uniq_1 (p{hr} - polyC (peval p{hr} i{hr}))
-            (edivpoly (p{hr} - polyC (peval p{hr} i{hr})) (X - polyC i{hr})).`1
-            (edivpoly p{hr} (X - polyC i{hr})).`1
-            (edivpoly (p{hr} - polyC (peval p{hr} i{hr})) (X - polyC i{hr})).`2
-            poly0
-            (X - polyC i{hr})).
-  + apply Xi_neq_0.
-  + apply degDiv_2. apply Xi_neq_0.
-  + smt(@BasePoly).
-  + apply polyRemThem_corr. apply Xi_neq_0.
-  + have h_prime := polyRemThem_corr p{hr} (X - polyC i{hr}) (Xi_neq_0 i{hr}).
-              rewrite -polyRemThem_r in h_prime.
-          smt(@BasePoly).
-  rewrite (polyRemThem_corr p{hr} (X - polyC i{hr})). apply Xi_neq_0.
-  rewrite -peval_add.
-  rewrite -(polyRemThem_corr p{hr} (X - polyC i{hr})). apply Xi_neq_0.
-  rewrite -polyRemThem_r.
-  rewrite peval_polyC. rewrite -peval_over_Xi. rewrite -peval_add.
-  rewrite peval_X. rewrite -peval_neg. rewrite peval_polyC.
-  pose crap := peval (edivpoly p{hr} (X - polyC i{hr})).`1 a.
-  have hd : crap * (a + - i{hr}) = crap * a - crap * i{hr}.
-  + rewrite Bl.ZP.ZModE.ZModpField.mulrC.
-    rewrite Bl.ZP.ZModE.ZModpField.mulrDl.
-    smt(@Bl.ZP.ZModE.ZModpField).
-  simplify. smt(@Bl.ZP.ZModE). *)
-qed. 
+  rewrite -Bl.ZP_GT.expD.
+  rewrite -Bl.ZP_GT.pow_bij.
+
+have hrem : (edivpoly (p{hr} - polyC (peval p{hr} i{hr})) (X - polyC i{hr})).`2 = poly0.
+  + have h1 := polyRemThem_r (p{hr} - polyC (peval p{hr} i{hr})) i{hr}.
+    have h2 : peval (p{hr} - polyC (peval p{hr} i{hr})) i{hr} = zero.
+    + smt(peval_add peval_neg peval_polyC @R).
+    smt(@BasePoly).
+
+have hdiv : p{hr} - polyC (peval p{hr} i{hr}) =
+    (edivpoly (p{hr} - polyC (peval p{hr} i{hr})) (X - polyC i{hr})).`1 * (X - polyC i{hr}).
+  + have := polyRemThem_corr (p{hr} - polyC (peval p{hr} i{hr})) (X - polyC i{hr}) (Xi_neq_0 i{hr}).
+    smt(@BasePoly).
+
+
+have heval : peval (p{hr} - polyC (peval p{hr} i{hr})) a =
+    peval (edivpoly (p{hr} - polyC (peval p{hr} i{hr})) (X - polyC i{hr})).`1 a *
+    peval (X - polyC i{hr}) a.
+  + have hxi := peval_over_Xi
+      (edivpoly (p{hr} - polyC (peval p{hr} i{hr})) (X - polyC i{hr})).`1 i{hr} a.
+    smt(@BasePoly).
+
+smt(peval_add peval_neg peval_polyC peval_X @R).
+
+qed.
 
 
 
 
-  
 
-   lemma not_inv (x : exp) : one - x <> - x. (*fixed*)
+
+
+
+
+
+
+
+
+
+
+
+
+
+
+   lemma not_inv (x : exp) : one - x <> - x.
        have : forall (a b c : exp), a <> c + b => a - b <> c.
        smt(@Bl.ZP.ZModE). move => h. apply h. smt(@Bl.ZP.ZModE).
      qed.
@@ -386,7 +394,7 @@ qed.
     }
   }.
 
-(*fixed*)
+
 lemma PolyComDLScheme_PolynomialBinding (A <: AdvPB) &m :
       Pr[PolynomialBinding(PolyComDLScheme, A).main() @ &m : res] <=
       Pr[Bl.Tsdh(Adv(A)).main() @ &m : res].
@@ -413,8 +421,7 @@ qed.
 
   
  
-    (* EvaluationBinding *) *)
-(*fixed*)
+    (* EvaluationBinding *)
 module Adv2 (Adv : AdvEB) : Bl.TsdhAdv = {
   proc comp(ga : Bl.GB.group list) : exp * Bl.GB.group = {
       var c, w, w' : Bl.GB.group;
@@ -427,6 +434,8 @@ module Adv2 (Adv : AdvEB) : Bl.TsdhAdv = {
     }
   }. 
 
+
+(*fixed*)
 lemma PolyComDLScheme_EvaluationBinding (A <: AdvEB) &m :
     Pr[EvaluationBinding(PolyComDLScheme, A).main() @ &m : res] <=
     Pr[Bl.Tsdh(Adv2(A)).main() @ &m : res].
@@ -470,33 +479,38 @@ rewrite (nth_mkseq). smt(Bl.t_valid). simplify.
 
     
   rewrite H1 in H2. rewrite Bl.GT_shuffle2 in H2. 
-  rewrite mkKey_ga in H2. rewrite -Bl.GT.expB in H2. (* rewrite Bl.GB.log_bij in H2. 
-  rewrite !Bl.exp_gt_eq in H2. *) rewrite -Bl.GP.expB in H2. rewrite Bl.GP.loggK in H2.
-   rewrite Bl.e_div1 in H2. rewrite Bl.log_e_gen in H2.  rewrite Bl.GB.logK in H2. rewrite -H2. smt(@Bl.ZP Bl.GB.g)
-  rewrite -(Bl.GPB.expgK (Bl.GB.(/) result_R.`4 result_R.`6)).
-  rewrite -Bl.exp_gb_eq. rewrite -Bl.GB.expM. apply Bl.exp_GB_can2.
-  apply Bl.GP.pow_bij. rewrite Bl.exp_gb_eq. rewrite Bl.GPB.expgK.
-  rewrite !Bl.GP.ZModE.asintK. move => @/Bl.GPB.loge.
-  rewrite Bl.GPB.ZModE.inzmodK. rewrite Bl.order_eq.
-  rewrite !Bl.GP.ZModE.inzmodM. rewrite -!Bl.GP.ZModE.inzmodK.
-  rewrite !Bl.GP.ZModE.inzmodB. rewrite !Bl.GP.ZModE.asintK.
-  pose x := Bl.GB.log (Bl.GB.(/) result_R.`4 result_R.`6).
-  (* need to show x is non zero *)
-  have : inzmod x <> zero. have : result_R.`4 <> result_R.`6. apply (contraNneq false).
-  move => h'''. apply H0. have : (result_R.`5 - result_R.`3 = zero => result_R.`3 = result_R.`5).  smt(@Bl.GP.ZModE).
-  move => g.  apply g.  rewrite -H2. rewrite h'''. smt(@Bl.GP.ZModE @Bl.GB). trivial.  move => h'''.
-  move => @/x.  apply (contraNneq false). move => g. apply h'''. apply Bl.GB_zero. rewrite Bl.eq_inzmod in g.
-  smt(@Bl.GB Bl.order_eq). smt(Bl.prime_q). smt(@Bl.GB). trivial. move => g.
-  (* resuming *)
-  rewrite !Bl.GP.ZModE.ZModpField.mul1r.
-  rewrite Bl.GP.ZModE.ZModpField.invrM. trivial. smt(@Bl.GP.ZModE). 
-  rewrite (Bl.GP.ZModE.ZModpField.mulrC _ (inv (inzmod x))).
-  rewrite Bl.GP.ZModE.ZModpField.mulrA. rewrite Bl.GP.ZModE.ZModpField.divrr. trivial.
-  smt(@Bl.GP.ZModE).
-  (* misc *) 
-      smt(). smt().
+      rewrite mkKey_ga in H2.
 
 
+ 
+      rewrite -Bl.ZP_GT.expB in H2.
+
+
+    rewrite -Bl.ZP.expB in H2. 
+
+  rewrite Bl.e_div1 in H2.
+pose R   := Bl.GB.( * ) result_R.`4 (Bl.GB.inv result_R.`6).
+pose a   := aL - result_R.`2.
+pose b   := result_R.`5 - result_R.`3.
+
+
+
+have hRa : R ^ a = Bl.GB.g ^ b.
++ apply (Bl.e_inj1 _ _ Bl.GB.g); first exact Bl.g_neq_e.
+  rewrite !Bl.e_pow1 Bl.e_g_g -Bl.e_pow2.
+  exact H2.
+
+have nz_a : a <> Bl.ZP.ZModE.zero by rewrite /a; smt(@Bl.ZP.ZModE).
+have nz_b : b <> Bl.ZP.ZModE.zero by rewrite /b; smt(@Bl.ZP.ZModE).
+pose xR := Bl.ZP.loge R.
+have hRexp : R = Bl.GB.g ^ xR by rewrite /xR Bl.ZP.expgK.
+
+have hxR : Bl.ZP.ZModE.( * ) xR a = b.
++ have := hRa. rewrite {1}hRexp -Bl.ZP.expM. by move/Bl.exp_GB_can.
+
+rewrite hRexp -Bl.ZP.expM.
+  apply Bl.exp_GB_can.
+smt(@Bl.ZP.ZModE @Bl.ZP.ZModE.ZModpField).
 
     smt ().
 smt().
@@ -649,33 +663,63 @@ module Adv3 (Adv : AdvH) : Bl.TsdhAdv = {
 }.
 
 
+(*fixed*)
 lemma Ad3_bad_prob &m :
   Pr[HidingWithBad(A).main() @ &m : HidingWithBad.bad] <= Pr[Bl.Tsdh(Adv3(A)).main() @ &m : res] .
-proof. admit. (*
+proof. 
   byequiv. proc. inline *. swap{1} 1 2. seq 4 6 : (={glob A, a,key,phi} /\ c{1} = c0{2} /\ d{1} = d0{2} /\ ga{2} = Bl.mkKey a{2}).
   auto. progress. wp. call(_:true).
 while( ={a, key, phi, j,ws,phiis,js } /\ c{1} = c0{2} /\ d{1} = d0{2} /\ HidingWithBad.bad{1} = a{1} \in js{1}).
   auto. progress. auto. call(_:true). auto. progress. rewrite nth_mkseq. smt(Bl.t_valid). simplify.
   (* now to show equivlants of condiitions *)
   have : exp a{2} 1 = a{2}. smt(@Bl.ZP.ZModE). move => g. rewrite g.
-  pose x := nth zero result_R  (find (fun (x : Bl.ZP.exp) => Bl.GB.g ^ asint x = Bl.GB.g ^ asint a{2}) result_R).
-  have : x = a{2}. have : Bl.GB.g ^ asint x  = Bl.GB.g ^ asint a{2}. smt(@List). smt(@Bl).
-  move => h''. rewrite h''. smt(@Bl.GP.ZModE.ZModpField). rewrite nth_mkseq. smt(Bl.t_valid).
-  have : exp a{2} 1 = a{2}. smt(@Bl.GP.ZModE). move => g. simplify. rewrite g.
-   pose x := nth zero result_R  (find (fun (x : Bl.GP.exp) => Bl.GB.g ^ asint x = Bl.GB.g ^ asint a{2}) result_R).
-   have : x = a{2}. have : Bl.GB.g ^ asint x  = Bl.GB.g ^ asint a{2}. smt(@List). smt(@Bl).
-   move => h''. rewrite h''. have : a{2} + (one - a{2}) = one. smt(@Bl.GP.ZModE.ZModpField). move => g'. rewrite g'.
-      smt(@Bl.GB @Bl.GP.ZModE). smt().  smt().  *)
+  pose x := nth zero result_R  (find (fun (x : Bl.ZP.exp) => Bl.GB.g ^ x = Bl.GB.g ^ a{2}) result_R).
+  have : x = a{2}. have : Bl.GB.g ^ x  = Bl.GB.g ^ a{2}. smt(@List). smt(@Bl).
+  move => h''. rewrite h''. smt(@Bl.ZP.ZModE.ZModpField). rewrite nth_mkseq. smt(Bl.t_valid).
+  have : exp a{2} 1 = a{2}. smt(@Bl.ZP.ZModE). move => g. simplify. rewrite g.
+   pose x := nth zero result_R  (find (fun (x : Bl.ZP.exp) => Bl.GB.g ^ x = Bl.GB.g ^ a{2}) result_R).
+   have : x = a{2}. have : Bl.GB.g ^ x  = Bl.GB.g ^ a{2}. smt(@List). smt(@Bl).
+   move => h''. rewrite h''. have : a{2} + (one - a{2}) = one. smt(@Bl.ZP.ZModE.ZModpField). move => g'. rewrite g'.
+      smt(@Bl.GB @Bl.ZP.ZModE). smt().  smt(). 
 qed. 
   
-(* we have now dealt with the case where the adverary learns an evaluation point from the key *)
+    (* we have now dealt with the case where the adverary learns an evaluation point from the key *)
+
+
+
+
+
+
+
+(*fixed*)
 lemma real_bad &m :
     Pr[Hiding(PolyComDLScheme, A).real() @ &m : res] = Pr[HidingWithBad(A).main() @ &m : res].
-proof. admit. (*
-  byequiv. proc. call(_:true). while(={j,ws,key,phi,js}). inline *. auto. progress. auto. call(_:true). inline*. auto. progress.
-  trivial.*) qed.
+proof.
+  byequiv => //. proc. inline *.
+  wp. call (_: true).
+  while (={j, ws, key, phi, js, phiis}).
+  - wp; skip => /> &2.
+    pose i := nth zero js{2} j{2}.
+    have h_adj := polyRemThem_adj phi{2} i.
+    have h_r   := polyRemThem_r   phi{2} i.
+    have heq :
+      phi{2} - polyC (peval phi{2} i)
+      = (edivpoly phi{2} (X - polyC i)).`1 * (X - polyC i)
+      by rewrite h_r; exact h_adj.
+    have hquot :
+      (edivpoly (phi{2} - polyC (peval phi{2} i)) (X - polyC i)).`1
+      = (edivpoly phi{2} (X - polyC i)).`1.
+    + rewrite heq. apply ediv_mul_qut. apply Xi_neq_0.
+    smt().
+        wp.
+       wp. call (_: true). wp. rnd. wp. rnd. skip. progress.
 
-module AdvHtoDL : Bl.DLogAdv ={
+qed.
+
+
+
+  (*fixed*)
+module AdvHtoDL (A : AdvH) : Bl.DLogAdv = {
   proc guess(ga : Bl.GB.group) = {
     var a, key; (* The secret and commitment scheme key *)
       var i, phii : exp; (* Adversary's response *)
@@ -695,7 +739,7 @@ module AdvHtoDL : Bl.DLogAdv ={
       ws <- [];
       j <- 0;
       while (j < Bl.t -1) {
-        temp2 <- (Bl.GB.(/) ga (Bl.GB.g^ (asint (nth zero phiis j))))^(asint (one/(a-(nth zero js j))));
+        temp2 <- (Bl.GB.(/) ga (Bl.GB.g^  (nth zero phiis j)))^(one/(a-(nth zero js j)));
           ws <- temp2 :: ws;
         j <- j + 1;      
       }
@@ -708,11 +752,62 @@ module AdvHtoDL : Bl.DLogAdv ={
   }
 }.
 
+(*taken from addPoly*)
+axiom interpolate_prob3 phi j js : mu1 (dpoly Bl.t Bl.FD.dt) phi =
+mu1 (dlet Bl.FD.dt (fun x0 => dmap (dlist Bl.FD.dt (Bl.t - 1))
+  (fun (phiis'0 : Bl.ZP.exp list) => (x0, phiis'0)))) (peval phi j, map (peval phi) js).
+
+(*taken from addPoly*)
+lemma interpolate_in_dpoly js phis t : size js = t => size phis = t =>
+    interpolate js phis \in dpoly t Bl.FD.dt.
+proof.
+move => h0 h1. rewrite supp_dpoly. smt(@List). split. rewrite -h0. apply interpolate_deg; trivial. smt(). smt(@Poly @Bl.FD).
+qed.
+
+
+(*taken from addPoly*)
+lemma interpolate_corr2 js phiis : uniq js => size js = size phiis => map (fun x => peval (interpolate js phiis) x) js = phiis.
+    move => h h'. pose phi := interpolate js phiis. rewrite eq_sym. apply interpolate_corr; trivial.
+    apply interpolate_deg; trivial.
+qed.
+
+(*taken from addPoly*)
+lemma interpolate_corr2_head j js phi phis :  uniq (j :: js) => size js = size phis =>
+    peval (interpolate (j :: js) (phi :: phis)) j = phi.
+    move => h h'. have : map (peval (interpolate (j :: js) (phi :: phis))) (j :: js) =  (phi :: phis).
+    apply interpolate_corr2; trivial. smt(@List). simplify.  move => g. smt().
+qed.
+
+
+
+
+(*taken from addPoly*)
+lemma interpolate_corr2_tail j js phi phis :  uniq (j :: js) => size js = size phis =>
+    map (fun x => peval (interpolate (j :: js) (phi :: phis)) x) js = phis.
+    move => h h'. have : map (peval (interpolate (j :: js) (phi :: phis))) (j :: js) =  (phi :: phis).
+    apply interpolate_corr2; trivial. smt(@List). simplify.  move => g. smt().
+qed.
+
+
+(*taken form addPoly*)
+lemma inter_inter j j' js js' x phii : size js = size phii => size js' = size phii => uniq (j :: js) =>
+    interpolate (j :: js) (map (peval (interpolate (j' :: js') (x :: phii))) (j :: js)) =
+    interpolate (j' :: js') (x :: phii).
+proof.
+  move => h0 h1 h2. apply interpolate_corr; trivial. smt(interpolate_deg). smt(@List).
+qed.
+
+
+
+(*fixed*)
 lemma HidingWithBadEquiv &m :
     Pr[HidingWithBad2(A).main() @ &m : res /\ !HidingWithBad2.bad] =
     Pr[HidingWithBad(A).main() @ &m : res /\ !HidingWithBad.bad].
-proof. 
-  byequiv. proc. inline *. swap{1} 8 -5. swap{2} [2..3] -1. seq 3 2 : (={glob A, a, key} /\ key{1} = Bl.mkKey a{1} /\
+    proof.
+
+
+
+      byequiv. proc. inline *. swap{1} 8 -5. swap{2} [2..3] -1. seq 3 2 : (={glob A, a, key} /\ key{1} = Bl.mkKey a{1} /\
   size js'{1} = Bl.t-1 /\ uniq (a{1} :: js'{1})). rnd{1}. auto.
   progress. apply js'_sample_ll. apply (js'_sample_size aL); trivial. smt(js'_uniq @List). smt(js'_uniq @List).
 
@@ -724,7 +819,10 @@ proof.
   (fun x=> (peval x a{1}, map (peval x) js'{1})) : 0 0. auto. progress.
   (* poly to list to poly *) rewrite eq_sym. apply interpolate_corr. rewrite dmap_id in H2.
   rewrite supp_dpoly in H2. smt(Bl.t_valid). smt(@List). smt(@List). smt(@List). smt().
-  (* poly to list poly prob *) rewrite dmap_id. apply interpolate_prob3. 
+    (* poly to list poly prob *) rewrite dmap_id.
+
+
+    apply interpolate_prob3. 
   (* poly to list poly prob *) rewrite dmap_id. apply interpolate_in_dpoly. smt(@List).
   have :  xphiis'L.`2 \in dlist Bl.FD.dt (Bl.t - 1). clear H2 H3. rewrite supp_dlet in H4. smt(@Distr).
   move => g. smt(@List @DList Bl.t_valid). 
@@ -741,70 +839,208 @@ proof.
   HidingWithBad2.bad{1} = HidingWithBad.bad{2} /\
     key{1} = (Bl.mkKey a{1})%Bl /\ uniq (a{1} :: js'{1}) /\ size js'{1} = Bl.t - 1). auto. progress.
   auto. auto. auto.
-qed.
+  qed.
+
+
+(*taken form add Poly*)
+lemma inter_inter_tail a x js js'0 phi : size js'0 = size phi => size js = size phi =>
+    uniq (a :: js) => uniq (a :: js'0) =>
+    interpolate (a :: js) (x :: map (peval (interpolate (a :: js'0) (x :: phi))) js) =
+    interpolate (a :: js'0) (x :: phi).
+ proof.
+  admit.
+ qed.
+  
+
+
+
+
 
 lemma d_log &m :
- islossless A.guess =>  
- Pr[HidingWithBad2(A).main() @ &m : res /\ !HidingWithBad2.bad] <= Pr[Bl.DLogExp(AdvHtoDL).main() @ &m : res].
-proof.
+
+  islossless A.guess =>  
+
+  Pr[HidingWithBad2(A).main() @ &m : res /\ !HidingWithBad2.bad] <= 
+
+  Pr[Bl.DLogExp(AdvHtoDL(A)).main() @ &m : res].
+
+
+
+  proof.
+
+   
+
+   
   move => h. byequiv. proc. inline *. swap{2} [1..2] 2.
+
   seq 2 2 : (={glob A, a,key} /\ key{1} = Bl.mkKey a{1}). auto.
 
-  seq 3 3 : (={glob A, a,key,x,ga,js} /\ key{1} = Bl.mkKey a{1}  /\ ga{2} = Bl.GB.g ^ asint x{2}).
+
+
+  seq 3 3 : (={glob A, a,key,x,ga,js} /\ key{1} = Bl.mkKey a{1}  /\ ga{2} = Bl.GB.g ^  x{2}).
+
   auto. call (_:true). auto.
 
+
+
    (* stupid case 2 *)
+
   case (a{1} \in js{1}). wp. call{1} (_ : true ==> true). call{2} (_ : true ==> true).
+
   while (={j}). auto. wp. rnd{1}. auto. progress. apply js'_sample_ll. trivial. trivial.
 
+
+
   (* stupid case 1 *)
+
   case (size js{1} <> Bl.t-1). wp. call{1} (_ : true ==> true). call{2} (_ : true ==> true).
+
   while (={j}). auto. wp. rnd{1}. auto. progress. trivial. apply js'_sample_ll. trivial.
 
+
+
   (* stupid case 3*)
+
   case (! uniq js{1}). wp. call{1} (_ : true ==> true). call{2} (_ : true ==> true).
+
   while (={j}). auto.  wp. rnd{1}. auto. progress. trivial.  apply js'_sample_ll. trivial. 
 
+
+
   (* The first issue is to show the evaluation of the polynomials is equvilant *)
-  seq 5 1 : (={glob A, a,key,x,ga,js,phiis} /\ key{1} = Bl.mkKey a{1}  /\ ga{2} = Bl.GB.g ^ asint x{2} /\
+
+  seq 5 1 : (={glob A, a,key,x,ga,js,phiis} /\ key{1} = Bl.mkKey a{1}  /\ ga{2} = Bl.GB.g ^ x{2} /\
+
   ! (a{1} \in js{1}) /\ size js{1} = Bl.t - 1 /\ uniq (a{1} :: js'{1}) /\ size phiis{1} = Bl.t-1 /\
+
   phi{1} = interpolate (a{2} :: js'{1}) (x{2} :: phiis'{1}) /\ size js'{1} = Bl.t-1 /\ size phiis'{1} = Bl.t - 1
+
   /\ uniq js{1} /\ phiis{2} = map (peval (interpolate (a{1} :: js'{1})(x{1} :: phiis'{1}))) js{1}). swap{1} 1 2.  wp.
 
+
+
+
+
+  (* 1. Perform the random transformation *)
+
+
+
+
+
+
+
+
+
+
+
   rnd (fun phiis=> map (peval (interpolate (a{1}::js'{1})(x{1}::phiis))) js{1})
+
   (fun phiis => map (peval (interpolate (a{1} :: js{1})(x{1} :: phiis))) js'{1}). auto. progress.
 
-   apply js'_sample_ll.
-  (* left right left *) rewrite inter_inter_tail. smt(@DList Bl.t_valid). smt(@DList Bl.t_valid js'_sample_size). 
-    smt(js'_uniq). smt(@List). rewrite interpolate_corr2_tail. smt(@List). smt(@DList Bl.t_valid). trivial.
-  (* right left right prob in *) rewrite !(AddDistr.dlist_mu1 _ _ Bl.GT.order). smt(@DList Bl.t_valid). smt(@Bl.FD).
+
+
+    apply js'_sample_ll.
+
+    (* left right left *) rewrite inter_inter_tail.
+smt(js'_sample_size size_map @DList @List).
+
+
+ smt(@DList Bl.t_valid js'_sample_size @List). 
+
+    smt(js'_uniq). smt(@List). rewrite interpolate_corr2_tail. smt(@List). smt(@DList Bl.t_valid @List). trivial.
+
+  (* right left right prob in *) rewrite !(AddDistr.dlist_mu1 _ _ Bl.GT.order). smt(@DList Bl.t_valid @List). smt(@Bl.FD).
+
     smt(@List js'_sample_size). smt(@Bl.FD). trivial. apply supp_dlist. smt(Bl.t_valid). split. smt(@List). apply allP. smt(@Bl.FD).
-  (* right left right *) rewrite inter_inter_tail. smt(js'_sample_size @DList Bl.t_valid). smt(@DList Bl.t_valid). 
-  smt(@List). smt(js'_uniq). rewrite interpolate_corr2_tail. smt(js'_uniq). smt(js'_sample_size @DList Bl.t_valid). trivial.
+
+  (* right left right *) rewrite inter_inter_tail. smt(js'_sample_size @DList Bl.t_valid @List). smt(@DList Bl.t_valid @List). 
+
+  smt(@List). smt(js'_uniq). rewrite interpolate_corr2_tail. smt(js'_uniq). smt(js'_sample_size @DList Bl.t_valid @List). trivial.
+
     smt(js'_uniq). smt(js'_uniq). smt(@List). smt(js'_sample_size). smt(@List js'_sample_size).
 
+
+
   (* witnesses *)
-  wp. call(_:true). while (={glob A,  a, key, js, x, ga, phiis,j,ws} /\ key{1} = Bl.mkKey a{1} /\ ga{2} = Bl.GB.g ^ asint x{2} /\
+
+  wp. call(_:true). while (={glob A,  a, key, js, x, ga, phiis,j,ws} /\ key{1} = Bl.mkKey a{1} /\ ga{2} = Bl.GB.g ^  x{2} /\
+
   size js{1} = Bl.t -1 /\ 0 <= j{1} /\ ! (a{1} \in js{1}) /\ phi{1} = interpolate (a{1} :: js'{1}) (x{1} :: phiis'{1}) /\
+
     uniq js{1} /\ size phiis{1} = Bl.t -1 /\ size js'{1} = Bl.t-1 /\ size phiis'{1} = Bl.t-1 /\ uniq (a{1} :: js'{1}) /\
+
    phiis{2} = map (peval (interpolate (a{1} :: js'{1})(x{1} :: phiis'{1}))) js{1}).
-    auto. progress. rewrite comPolEval. apply degDiv2. smt(interpolate_deg). 
-  rewrite -Bl.GB.expB. rewrite -Bl.GB.expM. apply Bl.exp_GB_can2. apply Bl.GP.pow_bij. rewrite Bl.GP.ZModE.asintK.
-  rewrite Bl.GP.ZModE.inzmodM. rewrite Bl.GP.ZModE.inzmodB. rewrite !Bl.GP.ZModE.asintK. pose i := nth zero js{2} j{2}.
-  have : a{2} <> i. smt(@List). move => g. rewrite prt_eval. smt(@Bl.GP.ZModE). congr. rewrite interpolate_corr2_head.
-  smt(@List). smt(@List). smt(@List). smt(@Bl.GP.ZModE). smt().
 
-  auto. progress. rewrite H18. have : (peval (interpolate (a{2} :: js'{1}) (x{2} :: phiis'{1})) result_R.`1 :: 
-    map (peval (interpolate (a{2} :: js'{1}) (x{2} :: phiis'{1}))) js{2}) =
-    map (peval (interpolate (a{2} :: js'{1}) (x{2} :: phiis'{1}))) (result_R.`1::js{2}). smt(@List). move => g. rewrite g.
-    rewrite inter_inter. smt(). smt(). smt(). apply interpolate_corr2_head. smt(). smt(). trivial. trivial.
-qed.
+    auto. progress. rewrite comPolEval. apply degDiv2. smt(interpolate_deg).
 
-lemma PolyComDLScheme_Hiding  &m :
- islossless A.guess =>   
- Pr[Hiding(PolyComDLScheme, A).real() @ &m : res] <=
- Pr[Bl.DLogExp(AdvHtoDL).main() @ &m : res] + Pr[Bl.Tsdh(Adv3(A)).main() @ &m : res].
- proof.
+
+    rewrite -Bl.ZP.expB. 
+
+rewrite (nth_map zero zero); first by smt().
+
+  rewrite -Bl.ZP.expM.
+
+apply Bl.exp_GB_can.
+
+
+pose i := nth zero js{2} j{2}.
+
+
+have a_neq_i : (-i) + a{2} <> Bl.ZP.ZModE.zero
+  by rewrite /i; smt(@List @Bl.ZP.ZModE).
+
+
+rewrite prt_eval; first exact a_neq_i.
+
+have hINT_a :
+  peval (interpolate (a{2} :: js'{1}) (x{2} :: phiis'{1})) a{2} = x{2}.
++ apply interpolate_corr2_head; smt(@List).
+rewrite hINT_a.
+
+smt(@Bl.ZP.ZModE @Bl.ZP.ZModE.ZModpField).
+
+
+smt().
+
+auto.
+progress.
+
+have hlist :
+  result_R.`2 :: map (peval (interpolate (a{2} :: js'{1}) (x{2} :: phiis'{1}))) js{2}
+  = map (peval (interpolate (a{2} :: js'{1}) (x{2} :: phiis'{1})))
+        (result_R.`1 :: js{2}).
++ smt(@List).
+rewrite hlist.
+
+
+rewrite inter_inter.
++ smt(@List).
++ smt(@List).
++ smt(@List).
+apply interpolate_corr2_head.
++ smt(@List).
++ smt(@List).
+
+          trivial.
+        trivial.
+
+
+
+qed. 
+
+
+
+
+
+
+
+(*fixed*)
+lemma PolyComDLScheme_Hiding &m :
+  islossless A.guess =>   
+  Pr[Hiding(PolyComDLScheme, A).real() @ &m : res] <=
+  Pr[Bl.DLogExp(AdvHtoDL(A)).main() @ &m : res] + 
+  Pr[Bl.Tsdh(Adv3(A)).main() @ &m : res].
+proof.
  move => h. rewrite real_bad. have : forall (b a c : real), a <= b => b <= c => a <= c. smt(). move=> h'.
    apply (h' (Pr[HidingWithBad(A).main() @ &m : res /\ !HidingWithBad.bad] + Pr[HidingWithBad(A).main() @ &m : HidingWithBad.bad])).
    apply Ad3_split. have : forall (a a' b b':real), a <= a' => b <= b' => a + b <= a' + b'. smt().
@@ -813,4 +1049,7 @@ lemma PolyComDLScheme_Hiding  &m :
 
 
 end section Hiding.
+
+
+
 
